src/coq/ImpCorrectness.v
@@ -25,10 +25,41 @@ Open Scope list_scope.
 Require Import Program.
 
 
+Lemma rev_nil_inv : forall {A} (l:list A), rev l = [] -> l = [].
+Proof.
+  destruct l; intros; auto.
+  simpl in H.  apply app_eq_nil in H. destruct H. inversion H0.
+Qed.
+
+Lemma app_same_inv : forall {A} (l1 l2:list A), l1 = l2 ++ l1 -> l2 = [].
+Proof.
+  induction l1; intros l2 H.
+  - rewrite app_nil_r in H. auto.
+  - destruct l2; auto.
+    inversion H. subst.
+    assert ((l2 ++ a0 :: l1) = ((l2 ++ [a0]) ++ l1)).
+    rewrite <- app_assoc. simpl. reflexivity.
+    rewrite H0 in H2. apply IHl1 in H2. apply app_eq_nil in H2. inversion H2. inversion H3.
+Qed.  
+  
+Ltac simplify_lists :=
+  repeat (match goal with
+          | [H : ?x = ?y ++ ?x |- _ ] => apply app_same_inv in H
+          | [H : ?x = ?y ++ ?z ++ ?x |- _ ] => rewrite app_assoc in H
+          | [H : ?x ++ ?y = [] |- _ ] => apply app_eq_nil in H; let y := fresh in destruct H as [_ y]; inversion y
+          | [H : [] = ?x ++ [?y] |- _ ] => symmetry in H
+          | [H : [] <> [] |- _] => contradiction H
+          | [H : ?x::?l = [] |- _] => inversion H
+          | [H : [] = ?x::?l |- _] => inversion H
+          | [H : context[rev[]] |- _] => simpl in H
+          | [H : [] = [] |- _ ] => clear H
+          | [H : ?x = [] |- _ ] => subst
+          | [H : (_, _, _, inl _) = (_, _, _, inr _) |- _ ] => inversion H
+          end).
 
 (* Move to Compiler.v *)
-Ltac unfold_llvm H :=
-  progress (simpl in H; unfold llvm_bind in H; unfold llvm_ret in H; unfold lift in H).
+Ltac unfold_compiler H :=
+  progress (simpl in H; unfold cmd_bind in H; unfold cmd_ret in H; unfold exp_bind in H; unfold exp_ret in H; unfold lift_cmd in H; unfold lift_exp in H).
 
 Arguments Z.add _ _ : simpl nomatch.
 
@@ -95,7 +126,147 @@ Proof.
     apply IHb1 in H3. apply IHb2 in H5. rewrite H3. rewrite H5. reflexivity.
 Qed.  
 
+Definition list_le {A} (cd1 cd2 : list A) : Prop :=
+  exists cd, cd2 = cd ++ cd1.
 
+Lemma list_le_refl : forall {A} (cd:list A), list_le cd cd.
+Proof.
+  intros.
+  exists []. reflexivity.
+Qed.
+
+Lemma list_le_trans : forall {A} (cd1 cd2 cd3:list A), list_le cd1 cd2 -> list_le cd2 cd3 -> list_le cd1 cd3.
+Proof.
+  intros A cd1 cd2 cd3 H12 H23.
+  destruct H12 as [cd12 Heq12].
+  destruct H23 as [cd23 Heq23].
+  subst. exists (cd23 ++ cd12).
+  rewrite app_assoc. reflexivity.
+Qed.  
+
+Lemma list_le_antireflexive : forall {A} (l1 l2:list A), list_le l1 l2 -> list_le l2 l1 -> l1 = l2.
+Proof.
+  intros A l1 l2 H1 H2.
+  unfold list_le in H1.
+  unfold list_le in H2.
+  destruct H1 as [l3 Eq3].
+  destruct H2 as [l4 Eq4].
+  subst.
+  simplify_lists. reflexivity.
+Qed.
+
+Definition string_le (s t:string) : Prop := exists u, t = (u ++ s)%string.
+
+
+Inductive raw_id_le : raw_id -> raw_id -> Prop :=
+| id_Raw_Raw :
+    forall n m (Hlt: n <= m),
+      raw_id_le (Raw n) (Raw m)
+| id_Raw_Anon :
+    forall n m,
+      raw_id_le (Raw n) (Anon m)
+| id_Raw_Name :
+    forall n s,
+      raw_id_le (Raw n) (Name s)
+| id_Anon_Anon :
+    forall n m (Hlt: n <= m),
+      raw_id_le (Anon n) (Anon m)
+| id_Anon_Name :
+    forall n s,
+      raw_id_le (Anon n) (Name s)
+| id_Name_Name :
+    forall s t
+      (Hlt: string_le s t),
+      raw_id_le (Name s) (Name t)
+.                
+  
+Definition exp_state_le : (int * code) -> (int * code) -> Prop :=
+  fun '(n1,cd1) '(n2, cd2) => 
+  n1 <= n2 /\ list_le cd1 cd2.
+
+Lemma exp_state_le_refl: forall (s:int * code), exp_state_le s s.
+Proof.
+  intros. destruct s. simpl. split; auto. omega. apply list_le_refl.
+Qed.
+
+Lemma exp_state_le_trans : forall (s1 s2 s3:int * code), exp_state_le s1 s2 -> exp_state_le s2 s3 -> exp_state_le s1 s3.
+Proof.
+Admitted.
+
+Lemma exp_state_le_antireflexive : forall s1 s2, exp_state_le s1 s2 -> exp_state_le s2 s1 -> s1 = s2.
+Proof.
+Admitted.  
+
+
+
+Inductive  cmd_state_le : cmd_state -> cmd_state -> Prop :=
+| cmd_same_block :
+    forall n1 m1 is1 t1 bs1 n2 m2 is2 t2 bs2
+      (Hn: n1 <= n2)
+      (Hm: m1 <= m2)
+      (His: list_le is1 is2)
+      (Ht: t1 = t2)
+      (Hbs: bs1 = bs2),
+      cmd_state_le (mk_cs n1 m1 is1 t1 bs1) (mk_cs n2 m2 is2 t2 bs2)
+| cmd_new_block :
+    forall n1 m1 is1 t1 bs1 n2 m2 is2 t2 bs2
+      (Hn: n1 <= n2)
+      (Hm: m1 <= m2)
+      (Hcd: exists n, n1 <= n /\ n <= n2 /\ exists m, m1 <= m /\ m <= m2 /\
+            exists is', list_le ((mk_block (lid_of_Z n) [] (rev (is' ++ is1)) (IVoid m, t1))::bs1) bs2),
+      
+      cmd_state_le (mk_cs n1 m1 is1 t1 bs1) (mk_cs n2 m2 is2 t2 bs2)
+.
+
+Ltac exploit_cmd_state_le :=
+  repeat (match goal with
+          | [ H : cmd_state_le ?S1 ?S2 |- _ ] => destruct ?S1; destruct ?S2; inversion H; exploit_cmd_state_le
+          | [ H : exists b, _ |- _ ] => let X := fresh "c" in destruct H as [X H]; exploit_cmd_state_le
+          | [ H : ?a /\ ?b |- _ ] => let A := fresh "H" in destruct H as [A H]; exploit_cmd_state_le
+          end).
+
+
+Lemma cmd_state_le_refl : forall (cs:cmd_state), cmd_state_le cs cs.
+Proof.
+  destruct cs.
+  eapply cmd_same_block; eauto; try omega; try apply list_le_refl.
+Qed.  
+  
+
+Lemma cmd_state_le_trans : forall s1 s2 s3, cmd_state_le s1 s2 -> cmd_state_le s2 s3 -> cmd_state_le s1 s3.
+Proof.
+  intros s1 s2 s3 H12 H23.
+  destruct s1. destruct s2. destruct s3.
+  inversion H12; subst; auto.
+  - inversion H23; subst; auto.
+    + eapply cmd_same_block; eauto; try omega; try solve [eapply list_le_trans; eauto].
+    + exploit_cmd_state_le.
+      eapply cmd_new_block; eauto; try omega.
+      exists c. repeat split; try omega.
+      exists c0. repeat split; try omega.
+      destruct His as [is' H'].
+      exists (c1 ++ is').
+      subst. rewrite <- app_assoc. exact Hcd.
+  - inversion H23; subst; auto.
+    + exploit_cmd_state_le.
+      eapply cmd_new_block; eauto; try omega.
+      exists c. repeat split; try omega.
+      exists c0. repeat split; try omega.
+      exists c1. exact Hcd.
+    + exploit_cmd_state_le.
+      destruct Hcd as [cd' Hcd']. subst.
+      destruct Hcd0 as [cd0' Hcd0'].  subst.
+      eapply cmd_new_block; eauto; try omega.
+      exists c0. repeat split; try omega.
+      exists c3. repeat split; try omega.
+      exists c4. exists (cd0' ++
+     {| blk_id := lid_of_Z c; blk_phis := []; blk_code := rev (c2 ++ is0); blk_term := (IVoid c1, tm0) |}
+     :: cd').
+      simpl. rewrite <- app_assoc. reflexivity.
+Qed.      
+      
+
+(*
 Ltac compile_aexp_monotonic_case X :=
   match goal with [
   IHa1 : forall (n m : int) (code : list elt) (v : Ollvm_ast.value) (n' m' : int) (code' : list elt),
@@ -125,28 +296,28 @@ Ltac compile_aexp_monotonic_case X :=
     exists (I (IId (lid_of_Z n2')) (INSTR_Op (SV (OP_IBinop (X false false) i64 v1' v2'))) :: code2'' ++ code1'');
     simpl; rewrite app_assoc; reflexivity
   end.
-
+*)
                   
 Lemma compile_aexp_monotonic :
   forall g a
-    n m code (v : Ollvm_ast.value) n' m' code'
-    (Hcomp : compile_aexp g a (n,m,code) = ((n',m',code'),inr v)),
-    n <= n' /\ m <= m' /\   exists code'', code' = code'' ++ code.
+    s v s'
+    (Hcomp : compile_aexp g a s = (s',inr v)),
+    exp_state_le s s'.
 Proof.
   intros g a.
-  induction a; intros n1 m1 code1 v n2 m2 code2 Hcomp.  simpl in Hcomp.
-  - unfold_llvm Hcomp.
-    inversion Hcomp; subst. repeat split; try omega. exists []. simpl. reflexivity.
+  (* induction a; intros n1 m1 code1 v n2 m2 code2 Hcomp.  simpl in Hcomp. *)
+  (* - unfold_llvm Hcomp. *)
+  (*   inversion Hcomp; subst. repeat split; try omega. exists []. simpl. reflexivity. *)
 
-  - unfold_llvm Hcomp.
-    destruct (g i); simpl in Hcomp; try inversion Hcomp.
-    repeat split; try omega.
-    exists [I (IId (lid_of_Z n1)) (INSTR_Load false i64 (i64ptr, v0) None)]. simpl. reflexivity.
+  (* - unfold_llvm Hcomp. *)
+  (*   destruct (g i); simpl in Hcomp; try inversion Hcomp. *)
+  (*   repeat split; try omega. *)
+  (*   exists [I (IId (lid_of_Z n1)) (INSTR_Load false i64 (i64ptr, v0) None)]. simpl. reflexivity. *)
 
-  - compile_aexp_monotonic_case Add.
-  - compile_aexp_monotonic_case Sub.
-  - compile_aexp_monotonic_case Mul.
-Qed.    
+  (* - compile_aexp_monotonic_case Add. *)
+  (* - compile_aexp_monotonic_case Sub. *)
+  (* - compile_aexp_monotonic_case Mul. *)
+Admitted.
     
 
 Definition iid n (id:instr_id) : Prop := (IId (lid_of_Z n)) = id.
@@ -248,76 +419,7 @@ Proof.
 Qed.  
 
 
-(* AstProp.v *)
-Inductive straight : code -> Prop :=
-| straight_nil : straight []
-| straight_Op : forall id i tl
-    (IHS: straight tl)
-    (Hi: is_Op i),
-    straight ((id,i)::tl)
-| straight_Eff : forall id i tl
-    (IHS: straight tl)
-    (Hi: is_Eff i),
-    straight ((id,i)::tl)
-.             
-Hint Constructors straight.
-
-(* AstProp.v *)
-Lemma straight_app : forall cd1 cd2,
-    straight cd1 ->
-    straight cd2 ->
-    straight (cd1 ++ cd2).
-Proof.
-  intros cd1 cd2 H H0.
-  generalize dependent cd2.
-  induction H; intros cd2 H0; simpl; auto; try solve [constructor; eauto].
-Qed.  
-
-(* Excludes labels and terminators *)
-Inductive compiled_code : list elt -> code -> Prop :=
-| cc_nil : compiled_code [] []
-
-| cc_cons_Op : forall id i tl cd
-    (IHs: compiled_code tl cd),
-    compiled_code ((I id i)::tl) ((id, i)::cd)
-.    
-Hint Constructors compiled_code.
-
-Lemma compiled_code_app : forall x1 cd1 x2 cd2,
-    compiled_code x1 cd1 ->
-    compiled_code x2 cd2 ->
-    compiled_code (x1++x2) (cd1++cd2).
-Proof.
-  intros x1 cd1 x2 cd2 H.
-  revert x2 cd2.
-  induction H; intros x2 cd2 H0; simpl; auto; try solve [constructor; eauto].
-Qed.  
-
-(*
-(* AstProp.v *)
-Inductive pc_prefix (p:pc) (cd:code) : Prop :=
-| pc_prefix_intro :
-    forall cd'
-      (H: fetch p = cd ++ cd'),
-      pc_prefix p cd.
-
-(* AstProp.v *)
-Lemma pc_prefix_app :
-  forall p cd1 cd2
-    (HP: pc_prefix p (cd1 ++ cd2)),
-    pc_prefix p cd1.
-Proof.
-  intros p cd1.
-  destruct cd1; intros cd2 HP. 
-  - inversion HP. simpl in H.
-    eapply pc_prefix_intro. simpl. apply H.
-  - simpl in HP.
-    inversion HP.
-    simpl in H.
-    eapply pc_prefix_intro. simpl. rewrite <- app_assoc in H.
-    apply H.
-Qed.  
- *)
+(* Relational step semantics ------------------------------------------------ *)
 
 (*
   Holds if the machine runs in zero or more steps to a configuration that satisfies R
@@ -362,141 +464,6 @@ Proof.
   - eapply step_jump; eauto.
 Qed.    
     
-(*
-(* AstProp.v *)
-Definition pc_app (p:pc) (c:code) :=
-  let b := bk p in
-  mk_pc (fn p) (mk_block (blk_id b) (blk_phis b) ((blk_code b) ++ c) (blk_term b)).
-
-(* AstProp.v *)
-Lemma pc_app_nil :
-  forall (p:pc) (c:code)
-    (Hnil : fetch p = []),
-    fetch (pc_app p c) = c.
-Proof.
-  intros.
-  destruct p.
-  destruct bk0. unfold fetch in *. simpl in *.
-  subst. reflexivity.
-Qed.    
-
-
-Lemma pc_app_slc :
-    forall fn bid phis term,
-      let slc := slc_pc fn bid phis term in
-      forall cd1 cd2,
-        pc_app (slc cd1) cd2 = slc (cd1 ++ cd2).
-Proof.
-  intros fn bid phis term slc cd1 cd2. reflexivity.
-Qed.
-
-Lemma fetch_slc :
-  forall fn bid phis term,
-    let slc := slc_pc fn bid phis term in
-    forall cd,
-      fetch (slc cd) = cd.
-Proof.
-  intros fn0 bid phis term slc cd.
-  reflexivity.
-Qed.
-
-Lemma pc_prefix_id :
-    forall fn bid phis term,
-      let slc := slc_pc fn bid phis term in
-      forall cd,
-        pc_prefix (slc cd) cd.
-Proof.
-  intros fn bid phis term slc cd.
-  apply pc_prefix_intro with (cd' := []).
-  rewrite app_nil_r. reflexivity.
-Qed.  
-*)  
-
-(*
-Lemma step_code_app :
-  forall CFG fn bid phis term,
-    let slc := slc_pc fn bid phis term in
-    forall R1 cd1 e1 k1 mem1 
-      (HS1 : step_code CFG R1 cd1 (slc cd1, e1, k1) mem1)
-      R2 cd2  
-      (HR1 : forall st mem, R1 st mem ->
-             (fetch (pc_of st)) = [] /\ step_code CFG R2 cd2 (pc_app (pc_of st) cd2, env_of st, stack_of st) mem),
-      step_code CFG R2 (cd1++cd2) (slc (cd1++cd2), e1, k1) mem1.
-Proof.
-  intros CFG fn bid phis term slc R1 cd1 e1 k1 mem1 HS1.
-  remember (slc cd1, e1, k1) as s1.
-  generalize dependent e1. revert k1.
-  induction HS1; intros k1 e1 Heqs1 R2 cd2 HR1. 
-  -  simpl.
-     destruct (HR1 s m) as [Hf HR2]; auto.
-     destruct s as [[pc2 e2] k2].
-     simpl in *.
-     inversion Heqs1. subst.
-     unfold slc in HR2. rewrite pc_app_slc in HR2. auto.
-
-  - simpl.
-    destruct s' as [[pc2 e2] k2]. subst.
-    assert (pc2 = slc cd) as Hpc2. eapply stepD_Op_inversion; eauto.
-    rewrite Hpc2 in HS.
-    apply step_tau with (s' := (slc (cd++cd2), e2, k2)); auto. 
-    + apply pc_prefix_id.
-    + replace (slc ((id, i) :: cd ++ cd2)) with (pc_app (slc ((id,i)::cd)) cd2).
-      replace (slc (cd ++ cd2)) with (pc_app (slc cd) cd2) by reflexivity.
-      eapply stepD_Op_weakening; auto.
-      reflexivity.
-    + eapply IHHS1; auto. rewrite Hpc2. reflexivity.
-
-  - simpl.
-    inversion Hi.
-    + assert (exists lid, id = IId lid /\ e = Alloca t (fun (a:value) => (slc cd, add_env lid a e1, k1))).
-      eapply stepD_Eff_Alloca_inversion. subst. apply HS.
-      destruct H0 as [lid [Hid Heq]].
-
-      apply step_eff with (e := (fmap (fun st => (pc_app (pc_of st) cd2, env_of st, stack_of st)) e))(m':=m')(v:=v)
-            (k:=fun a0 : value => (pc_app (slc cd) cd2, add_env lid a0 e1, k1)); auto.
-      * apply pc_prefix_id.
-      * replace (slc ((id, i) :: cd ++ cd2)) with (pc_app (slc ((id,i)::cd)) cd2).
-        eapply stepD_Eff_weakening; auto.
-        subst.
-        apply HS.
-        reflexivity.
-      * subst. simpl. 
-        simpl in HM. inversion HM. reflexivity.
-      * eapply IHHS1; auto. rewrite Heq in HM. inversion HM. subst. reflexivity.
-
-    + assert (exists lid a, id = IId lid /\ e = Load a (fun (dv:dvalue) => (slc cd, add_env lid dv e1, k1))).
-      eapply stepD_Eff_Load_inversion. subst. apply HS.
-      destruct H0 as [lid [addr [Hid Heq]]].
-
-      apply step_eff with (e := (fmap (fun st => (pc_app (pc_of st) cd2, env_of st, stack_of st)) e))(m':=m')(v:=v)
-            (k:=fun a0 : value => (pc_app (slc cd) cd2, add_env lid a0 e1, k1)); auto.
-      * apply pc_prefix_id.
-      * replace (slc ((id, i) :: cd ++ cd2)) with (pc_app (slc ((id,i)::cd)) cd2).
-        eapply stepD_Eff_weakening; auto.
-        subst.
-        apply HS.
-        reflexivity.
-      * subst. simpl. 
-        simpl in HM. inversion HM. reflexivity.
-      * eapply IHHS1; auto. rewrite Heq in HM. inversion HM. subst. reflexivity.
-
-    + assert (exists vid a dv, id = IVoid vid /\ e = Store a dv (fun _ => (slc cd, e1, k1))).
-      eapply stepD_Eff_Store_inversion. subst. apply HS.
-      destruct H0 as [vid [addr [dv [Hid Heq]]]].
-
-      apply step_eff with (e := (fmap (fun st => (pc_app (pc_of st) cd2, env_of st, stack_of st)) e))(m':=m')(v:=v)
-            (k:=fun _ => (pc_app (slc cd) cd2, e1, k1)); auto.
-      * apply pc_prefix_id.
-      * replace (slc ((id, i) :: cd ++ cd2)) with (pc_app (slc ((id,i)::cd)) cd2).
-        eapply stepD_Eff_weakening; auto.
-        subst.
-        apply HS.
-        reflexivity.
-      * subst. simpl. 
-        simpl in HM. inversion HM. reflexivity.
-      * eapply IHHS1; auto. rewrite Heq in HM. inversion HM. subst. reflexivity.
-Qed.
-*)        
   
 Definition env_extends (e e':env) : Prop :=
   forall op t dv, eval_op e t op = inr dv -> eval_op e' t op  = inr dv.
@@ -574,26 +541,6 @@ Proof.
     (* maybe cut down on cases from eval_expr to simplify for now. *)
 Admitted.    
 
-Lemma rev_nil_inv : forall {A} (l:list A), rev l = [] -> l = [].
-Proof.
-  destruct l; intros; auto.
-  simpl in H.  apply app_eq_nil in H. destruct H. inversion H0.
-Qed.  
-
-Ltac simplify_lists :=
-  repeat (match goal with
-          | [H : rev ?x = [] |- _] => apply rev_nil_inv in H; inversion H; subst; clear H
-          | [H : ?x ++ ?y = [] |- _ ] => apply app_eq_nil in H; let y := fresh in destruct H as [_ y]; inversion y
-          | [H : [] = ?x ++ [?y] |- _ ] => symmetry in H
-          | [H : [] <> [] |- _] => contradiction H
-          | [H : ?x::?l = [] |- _] => inversion H
-          | [H : [] = ?x::?l |- _] => inversion H
-          | [H : context[rev[]] |- _] => simpl in H
-          | [H : [] = [] |- _ ] => clear H
-          | [H : ?x = [] |- _ ] => subst
-          | [H : (_, _, _, inl _) = (_, _, _, inr _) |- _ ] => inversion H
-          | [H : (_, _, _, inr _) = (_, _, _, inl _) |- _ ] => inversion H                                                                      
-          end).
 
 
 Ltac simplify_step :=
@@ -656,24 +603,10 @@ Ltac instantiate_H :=
 
   | [ H : ?X ++ ?TL = ?Y ++ ?TL |- _ ] => apply app_inv_tail in H; subst
 
-  | [ H0 : compiled_code ?CD0 ?CDA0 ,
-      H1 : compiled_code ?CD1 ?CDA1 
-     |- exists cd_a, exists c_a,
-        (I (IId (?X)) (?INS)) :: ?CD0 ++ ?CD1 ++ ?CD = cd_a ++ ?CD /\ _
-    ] =>
-    exists ((I (IId (X)) (INS)) :: CD0 ++ CD1);
-    exists ((IId (X), INS) :: CDA0 ++ CDA1)
-
   | [ |- _ /\ _ ] => split; instantiate_H
                     
   | [ |- ?X :: ?A ++ ?B ++ ?C = (?X :: ?A ++ ?B) ++ ?C ] => simpl; rewrite app_assoc; reflexivity
 
-  | [ |- compiled_code ((I ?X ?INS)::_) ((?X, ?INS)::_) ] => econstructor
-
-  | [ H1 : compiled_code ?C1 ?CA1,
-      H2 : compiled_code ?C2 ?CA2
-      |- compiled_code (?C1 ++ ?C2) (?CA1 ++ ?CA2) ] => apply compiled_code_app; assumption
-                                                                                      
  end).
 
 Ltac exploit_CFG_code :=
@@ -737,50 +670,76 @@ Ltac solve_step_star :=
       eapply step_tau
   end.
 
+(*
+  lbl: 
+   pc0 i0
+   pc1 i1
+   ...
+
+ P pcN [...]
+   ...
+   pcM ....
+ Q?   
+*)
+
+(*
 Lemma compile_aexp_correct :
-  forall 
-    (a:aexp) (st:Imp.state) (ans:int64)
-    (HAexp: aeval st a = ans)
+  forall g a n cd0
+      (n', cd, inr v) = compile_aexp g a (n, cd0)
+      CFG_has_code_at CFG P p1 (rev cd)
+      memory_invariant g e mem1 st
+      exists s2,
+        step_star CFG (fun '(p2, e2, k2) mem =>
+                         memory_invariant g e2 mem1 st /\
+                         Rv64e (eval_op e' (Some (TYPE_I 64)) v) (aeval st a) /\
+                         mem = mem1 /\ env_extends e e' /\ 
+                         (P p2) /\  k2 = k1)
+                         
+              (fun '(pc', e', k') mem' =>
+                 memory_invariant g e' mem' st /\
 
-    (g:ctxt)
-    (n m:int) (cd:list elt)
-    (n' m':int) (cd':list elt)
-    (v : Ollvm_ast.value)
-    (Hcomp : compile_aexp g a (n,m,cd) = ((n',m',cd'),inr v)),
+                 env_extends e e' /\
+                 env_lt (fst cs') e' /\ k = k'
+              )
+*)
 
-  exists cd_a c_a,
-    cd' = cd_a ++ cd
-    /\ compiled_code cd_a c_a
-    /\ forall
-    (e:env)
-    (mem:memory) (Hlt:env_lt n e)
-    (HM: memory_invariant g e mem st),
-        forall (CFG : mcfg) (p:pc) (k:stack) (P:pc -> Prop)
-          (HCFG: CFG_has_code_at CFG P p (List.rev c_a)),
-          step_star CFG
-                    (fun '(pc', e', k') mem' =>
-                       P pc' /\
-                       memory_invariant g e' mem' st /\
-                       Rv64e (eval_op e' (Some (TYPE_I 64)) v) ans /\
-                       env_extends e e' /\
-                       env_lt n' e' /\ k = k'
-                    )
-                    (p, e, k) mem.
+Lemma compile_aexp_correct :
+  forall (a:aexp) (st:Imp.state) 
+    (g:ctxt) n0 cd0 n1 cd1 (v : Ollvm_ast.value)
+    (Hcomp : (n1, cd1, inr v) = compile_aexp g a (n0, cd0)),
+    exists cd2,
+      cd1 = cd2 ++ cd0 /\
+      forall           
+        (CFG : mcfg) P (p1:pc) (e:env) (k:stack) 
+        (Hcfg: CFG_has_code_at CFG P p1 (rev cd2))
+        (mem:memory) (* (Hlt:env_lt n0 e) *)
+        (HM: memory_invariant g e mem st),
+        step_star CFG
+                  (fun '(pc', e', k') mem' =>
+                     P pc' /\ (fn pc' = fn p1) /\
+                     memory_invariant g e' mem' st /\
+                     Rv64e (eval_op e' (Some (TYPE_I 64)) v) (aeval st a) /\
+                     env_extends e e' /\
+(*                     env_lt n1 e' /\ *)
+                     k = k'
+                  )
+                  (p1, e, k) mem.
 Proof.
+Admitted.
+(*
   intros a st ans HAexp.
   rewrite aeval_iff_aevalR in HAexp.
 
-  induction HAexp; intros g n m cd n' m' cd' v Hcomp; unfold_llvm Hcomp.
-  - inversion_clear Hcomp. 
-    exists []. exists [].
-    repeat split; auto.
-    + intros e mem Hlt HM.
-      intros CFG p k P HCFG.
-      simpl in HCFG.
-      exploit_CFG_code.
-      eapply step_zero.
+  induction HAexp; intros g cs cs' v Hcomp CFG fid P p HCFG e k mem Hlt HM. 
+  - simpl in Hcomp. unfold_llvm Hcomp. inversion Hcomp. 
+
+    inversion HCFG. subst.
+          eapply step_zero.
       repeat split; auto.  rewrite Int64.repr_signed; auto.
       weakening.
+      subst. simpl in *.
+      eapply step_zero.
+      repeat split; auto.  
 
   - unfold trywith in Hcomp.
     remember (g id) as X.
@@ -901,48 +860,195 @@ Lemma compile_bexp_correct :
                     (p, e, k) mem.
 Proof.
 Admitted.  
+*)
 
-
-
-Definition CFG_has_compilation_of CFG fid g cmd :=
-  exists n m cd cd_c n' m' cd' bid term blks,
-    compile_com g cmd (n,m,cd) = ((n',m',cd'), inr ())
-    /\ cd' = cd_c ++ cd
-    /\ blocks_of_elts bid cd_c (IVoid m', term) = inr blks
-    /\ CFG_fun_has_blocks CFG fid blks.
-               
-(*
-Lemma compile_com_correct :
-  forall (cmd:com) (k:Imp.cont) (st:Imp.state) cmd' k' st'
-    (HStep: cmd / k / st ==> cmd' / k' / st')
-    (g:ctxt) (CFG:mcfg) (fn:function_id)
-    s mem
-    (Hrelated: related_configuration g cmd k st fn s mem),
-    step_star CFG (fun s' mem' =>
-                      let '(pc', e', k') := s' in
-                      related_configuration g cmd' st' fn s' mem'
-                   )
-               s mem.
+Lemma compile_bexp_correct :
+  forall (b:bexp) (st:Imp.state) 
+    (g:ctxt) n0 cd0 n1 cd1 (v : Ollvm_ast.value)
+    (Hcomp : (n1, cd1, inr v) = compile_bexp g b (n0, cd0)),
+    exists cd2,
+      cd1 = cd2 ++ cd0 /\
+      forall           
+        (CFG : mcfg) P (p1:pc) (e:env) (k:stack) 
+        (Hcfg: CFG_has_code_at CFG P p1 (rev cd2))
+        (mem:memory) (* (Hlt:env_lt n0 e) *)
+        (HM: memory_invariant g e mem st),
+        step_star CFG
+                  (fun '(pc', e', k') mem' =>
+                     P pc' /\ (fn pc' = fn p1) /\
+                     memory_invariant g e' mem' st /\
+                     Rv1e (eval_op e' (Some (TYPE_I 1)) v) (beval st b) /\
+                     env_extends e e' /\
+(*                     env_lt n1 e' /\ *)
+                     k = k'
+                  )
+                  (p1, e, k) mem.
 Proof.
-  intros cmd res st st' Hceval.
-  induction Hceval; intros g CFG fn s mem Hrel; inversion Hrel; clear Hrel; subst; auto.
+Admitted.
 
-  - unfold_llvm Hcomp.
-    inversion Hcomp; subst.
-    eapply step_zero2. left.
-    split; auto.
-    destruct s as [[pc e] k].
-    simpl in Hpc.
-    rewrite <- app_nil_l in H2 at 1.
-    apply app_inv_tail in H2.
-    subst. simpl in *.
-    unfold blocks_of_elts in Hblks.
-    simpl in Hblks. inversion Hblks. subst.
-    exists m'. exists bid. exists term.
-    split; auto.
 
-  - unfold_llvm Hcomp.
-    remember (compile_aexp
+
+Inductive matching_state (CFG:mcfg) (g:ctxt) (fid:function_id) (P:pc -> Prop) : pc -> com -> Prop :=
+| match_skip:
+    forall p
+      (Hp: P p),
+      matching_state CFG g fid P p SKIP
+
+| match_assn:
+    forall p a x n v cd n' m ptr
+      (Ha: ((n',cd), inr v) = compile_aexp g a (n, []))
+      (Hx: (g x) = Some ptr)
+      (HCFG: CFG_has_code_at CFG P p (rev ((IVoid m, (INSTR_Store false (i64, v) (i64ptr, ptr) None))::cd))),
+      matching_state CFG g fid P p (CAss x a)
+
+| CSeq:
+    forall p q c1 c2 
+      (Hc1: matching_state CFG g fid (fun pc => pc = q) p c1)
+      (Hc2: matching_state CFG g fid P q c2),
+      matching_state CFG g fid P p (CSeq c1 c2) 
+                     
+| CIf:
+    forall p b n v cd n' br1 br2 merge c1 c2 p1 p2 pmerge
+      (Ha: ((n', cd), inr v) = compile_bexp g b (n, []))
+      (HCFG: CFG_has_code_at CFG (fun q => fetch CFG q = Some (Term (TERM_Br (i1, v) br1 br2)))
+                             p (rev cd))
+      (HBR1: CFG_fun_has_block_id CFG fid br1 p1)
+      (IH1: matching_state CFG g fid (fun q => fetch CFG q = Some (Term (TERM_Br_1 merge))) p1 c1)
+      (HBR2: CFG_fun_has_block_id CFG fid br2 p2)
+      (IH2: matching_state CFG g fid (fun q => fetch CFG q = Some (Term (TERM_Br_1 merge))) p2 c2)
+      (Hmerge: CFG_fun_has_block_id CFG fid merge pmerge)
+      (IHmerge: matching_state CFG g fid P pmerge SKIP),
+      matching_state CFG g fid P p (CIf b c1 c2)
+
+| CWhile:
+    forall p b n v cd n' body entry exit c pentry pbody pexit
+      (Hpcd: fetch CFG p = Some (Term (TERM_Br_1 entry)))
+      (Hentry: CFG_fun_has_block_id CFG fid entry pentry)
+      (Ha: ((n', cd), inr v) = compile_bexp g b (n, []))
+      (HCFG: CFG_has_code_at CFG (fun q => fetch CFG q = Some (Term (TERM_Br (i1, v) body exit)))
+                           pentry (rev cd))
+      (Hbody: CFG_fun_has_block_id CFG fid body pbody)
+      (IH1: matching_state CFG g fid (fun q => fetch CFG q = Some (Term (TERM_Br_1 entry))) pbody c)
+      (Hexit: CFG_fun_has_block_id CFG fid exit pexit)
+      (IHexit: matching_state CFG g fid P pexit SKIP),
+      matching_state CFG g fid P p (CWhile b c)
+.
+Hint Constructors matching_state.  
+
+
+Inductive related_configuration (CFG:mcfg) fid g (cmd:com) (st:Imp.state) (s:SS.state) (mem:memory) P : Prop :=
+| config_intro :
+    forall p e k
+    (Hs: s = (p, e, k))
+    (Hmem : memory_invariant g e mem st)
+    (Hcfg: matching_state CFG g fid P p cmd)
+    (Hpc: (fn p) = fid)
+    ,
+    related_configuration CFG fid g cmd st s mem P.
+Hint Constructors related_configuration.    
+
+Lemma compile_com_correct :
+  forall (cmd1 cmd2:com) (st1 st2:Imp.state)
+    (HStep: cmd1 / st1 ==> cmd2 / st2)
+    (g:ctxt) (CFG:mcfg) (fid:function_id) (s1:SS.state) (mem1:memory) P
+    (Hrel: related_configuration CFG fid g cmd1 st1 s1 mem1 P),
+    step_star CFG (fun s2 mem2 =>
+                     related_configuration CFG fid g cmd2 st2 s2 mem2 P
+                  )
+              s1 mem1.
+Proof.
+Admitted.
+(*
+  intros cmd1 cmd2 st1 st2 HStep.
+  induction HStep; intros.
+
+  - inversion Hrel. inversion Hcfg; subst.
+    simpl in HCFG.
+    exploit_CFG_code.
+    pose (compile_aexp_correct a1 st g n0 [] n' cd v ltac:(auto)) as K; clearbody K.
+    destruct K as [cd2 [Heqcd K]].
+    rewrite app_nil_r in Heqcd. subst.
+    pose (K CFG _ p e k HL mem1 ltac:(auto)) as HA; clearbody HA; clear K.
+    eapply step_star_app.
+    eapply HA.
+    intros [[pc2 e2] k2]. intros mem2. intros [Heq [Hfn [Hmem2 [Heval [Hext Hk2]]]]].
+    subst.
+      
+    inversion Heval. simplify_step.
+    unfold memory_invariant in Hmem2. 
+    apply Hmem2 in Hx.
+    destruct Hx. destruct H1. destruct H3. destruct H3.
+    subst. 
+
+    eapply step_eff.
+    simplify_step.
+    rewrite <- H0. simpl.
+      reflexivity.
+      reflexivity.
+      eapply step_zero.
+      eapply config_intro.
+      reflexivity.
+      unfold memory_invariant.
+      intros.
+      apply Hmem2 in H1.
+      destruct H1. destruct H1. destruct H2. destruct H2.
+      exists x3. repeat split; eauto.
+      exists x4. repeat split; auto.
+      subst. 
+      inversion Heval.
+      subst.
+      inversion H4.
+      unfold Rv64.
+      inversion H5.
+      (* Needs injectivity of g and some other facts about nth_default and replace *)
+      admit.
+
+      eauto. rewrite <- Hfn.
+
+  - inversion Hrel.
+    inversion Hcfg. subst.
+    
+    eapply step_star_app.
+    eapply IHHStep.
+    econstructor. reflexivity. eauto. apply Hc1.
+    intros [[pc2 e2] k2]. intros mem2 HR.
+    inversion HR. 
+    eapply step_zero.
+    econstructor.  exact Hs. eauto.
+    econstructor. eauto. eauto.
+
+  - inversion Hrel.
+    inversion Hcfg.
+    inversion Hc1. subst.
+    subst.
+    eapply step_zero.
+    econstructor; eauto.
+
+  - inversion Hrel.
+    inversion Hcfg.
+    subst.
+    eapply step_star_app.
+    pose (compile_bexp_correct b st g n [] n' cd v ltac:(auto)) as K; clearbody K.
+    destruct K as [cd2 [Heqcd K]].
+    rewrite app_nil_r in Heqcd. subst.
+    pose (K CFG _ p e k HCFG mem1 ltac:(auto)) as HA; clearbody HA; clear K.
+    eapply step_star_app.
+    eapply HA.
+    intros [[pc2 e2] k2]. intros mem2. intros [Heq [Hmem2 [Heval [Hext Hk2]]]].
+    subst.
+
+    eapply step_jump.
+    simplify_step.
+    inversion Heval. subst. unfold i1.  rewrite <- H0.
+    simpl. unfold Rv1 in H1.
+    destruct (beval st b).
+    subst. simpl.
+    unfold jump.
+    
+
+      
+      
+      
 
 
 Lemma compile_com_correct :
