src/coq/StepSemantics.v
@@ -825,9 +825,9 @@ Definition jump (CFG:mcfg) (fid:function_id) (bid_src:block_id) (bid_tgt:block_i
   in
   match find_block_entry CFG fid bid_tgt with
   | None => failwith ("jump: target block " ++ string_of bid_tgt ++ " not found")
-  | Some (BlockEntry phis pc_next) =>
+  | Some (BlockEntry phis pc_entry) =>
     'e_out <- monad_fold_right eval_phi phis e_init;
-      mret (pc_next, e_out, k)
+      mret (pc_entry, e_out, k)
   end.
 
 
@@ -959,7 +959,7 @@ Definition stepD (CFG:mcfg) (s:state) : transition state :=
 
     
 
-(* Assumes that the entry-point function is named "fn" and that it takes
+(* Assumes that the entry-point function is named "fname" and that it takes
    no parameters *)
 Definition init_state (CFG:mcfg) (fname:string) : err state :=
   'fentry <- trywith ("INIT: no function named " ++ fname) (find_function_entry CFG (Name fname));
