src/coq/CFG.v
@@ -88,10 +88,16 @@ Definition fallthrough (cd: code) term_id : instr_id :=
   end.
 
 Definition blk_term_id b := fst (blk_term b).
+Definition blk_terminator b := snd (blk_term b).
 
 Definition blk_entry_id (b:block) : instr_id := fallthrough (blk_code b) (blk_term_id b). 
 
-  
+Definition blk_entry_pc (fid:function_id) (b:block) :=
+  mk_pc fid (blk_id b) (blk_entry_id b).
+
+Definition blk_term_pc (fid:function_id) (b:block) :=
+  mk_pc fid (blk_id b) (blk_term_id b).
+
 Fixpoint find_block bs block_id : option block :=
   find (fun b => if (blk_id b) == block_id then true else false) bs.
 
@@ -105,12 +111,12 @@ Fixpoint find_instr (cd : code) (p:instr_id) (t:instr_id) : option (cmd * option
       find_instr cd p t
   end.
 
-Definition block_to_cmd (b:block) (p:instr_id) : option (cmd * option instr_id) :=
+Definition block_to_cmd (b:block) (iid:instr_id) : option (cmd * option instr_id) :=
   let term_id := blk_term_id b in 
-  if term_id == p then
+  if term_id == iid then
     Some (Term (snd (blk_term b)), None)
   else
-    find_instr (blk_code b) p term_id 
+    find_instr (blk_code b) iid term_id 
 .
                
 Definition fetch (CFG : mcfg) (p:pc) : option cmd :=
@@ -131,8 +137,8 @@ Definition incr_pc (CFG:mcfg) (p:pc) : option pc :=
 Inductive block_entry : Set :=
 | BlockEntry (phis:list (local_id * phi)) (p:pc).
 
-Fixpoint block_to_entry (fn:function_id) (b:block) : block_entry :=
-  BlockEntry (blk_phis b) (mk_pc fn (blk_id b) (blk_entry_id b)).
+Fixpoint block_to_entry (fid:function_id) (b:block) : block_entry :=
+  BlockEntry (blk_phis b) (blk_entry_pc fid b).
 
 Definition find_block_entry (CFG:mcfg) (fid:function_id) (bid:block_id) : option block_entry :=
   'cfg <- find_function CFG fid;
