src/coq/CFGProp.v
@@ -60,37 +60,25 @@ Proof.
     exists pc2. split; eauto.
 Qed.
 
+
 Definition CFG_has_pc (CFG:mcfg) (p:pc) : Prop :=
   exists cmd, fetch CFG p = Some cmd.
 
-Definition CFG_fun_has_block_id (CFG:mcfg) (fid:function_id) (bid:block_id) : Prop :=
-  exists phis p, find_block_entry CFG fid bid = Some (BlockEntry phis p) /\ CFG_has_pc CFG p. 
+Definition CFG_fun_has_block_id (CFG:mcfg) (fid:function_id) (bid:block_id) (p:pc) : Prop :=
+  exists phis, find_block_entry CFG fid bid = Some (BlockEntry phis p) /\ CFG_has_pc CFG p. 
 
-Inductive CFG_fun_has_block (CFG:mcfg) (fid:function_id) (b:block) : Prop :=
-| CFG_fun_has_trivial_block:
-    forall phis p
-      (HFind: find_block_entry CFG fid (blk_id b) = Some (BlockEntry phis p))      
-      (Hp : p = mk_pc fid (blk_id b) (blk_term_id b)),
-      CFG_fun_has_block CFG fid b
-
-| CFG_fun_has_nontrivial_block:
-    forall phis p
-      (HFind: find_block_entry CFG fid (blk_id b) = Some (BlockEntry phis p))
-      (Hbody: CFG_has_code_at CFG (fun pc => pc = mk_pc fid (blk_id b) (blk_term_id b))
-                              (mk_pc fid (blk_id b) (blk_entry_id b)) (blk_code b)),
-      CFG_fun_has_block CFG fid b.
 
 Inductive CFG_fun_has_terminator_lbls (CFG:mcfg) (fid:function_id) : terminator -> Prop :=
 | lbls_Ret : forall v, CFG_fun_has_terminator_lbls CFG fid (TERM_Ret v)
 | lbls_Ret_void : CFG_fun_has_terminator_lbls CFG fid TERM_Ret_void
 | lbls_TERM_Br :
-    forall v br1 br2
-      (Hbr1 : CFG_fun_has_block_id CFG fid br1)
-      (Hbr2 : CFG_fun_has_block_id CFG fid br2),
+    forall v br1 p1 br2 p2
+      (Hbr1 : CFG_fun_has_block_id CFG fid br1 p1)
+      (Hbr2 : CFG_fun_has_block_id CFG fid br2 p2),
       CFG_fun_has_terminator_lbls CFG fid (TERM_Br v br1 br2)
 | lbls_TERM_Br_1 :
-    forall br
-      (Hbr : CFG_fun_has_block_id CFG fid br),
+    forall br p
+      (Hbr : CFG_fun_has_block_id CFG fid br p),
       CFG_fun_has_terminator_lbls CFG fid (TERM_Br_1 br)
 | lbls_Resume : forall v, CFG_fun_has_terminator_lbls CFG fid (TERM_Resume v)
 .
@@ -100,6 +88,26 @@ Inductive CFG_fun_has_terminator_lbls (CFG:mcfg) (fid:function_id) : terminator 
   | TERM_Invoke     (fnptrval:tident) (args:list tvalue) (to_label:block_id) (unwind_label:block_id)
   .
 *)
+
+
+Inductive CFG_has_terminator_at (CFG:mcfg) : pc -> instr_id -> terminator -> Prop :=
+| CFG_has_termintator_intro :
+    forall p iid t
+      (HF: fetch CFG p = Some (Term t))
+      (Hiid: (pt p) = iid)
+      (Hbrs: CFG_fun_has_terminator_lbls CFG (fn p) t),
+      CFG_has_terminator_at CFG p iid t.
+
+
+Inductive CFG_fun_has_block (CFG:mcfg) (fid:function_id) (b:block) : Prop :=
+| CFG_fun_has_block_intro:
+    forall phis 
+      (HFind: find_block_entry CFG fid (blk_id b) = Some (BlockEntry phis (blk_entry_pc fid b)))      
+      (Hcode: CFG_has_code_at CFG (fun q => q = blk_term_pc fid b) (blk_entry_pc fid b) (blk_code b))
+      (Hterm: CFG_has_terminator_at CFG (blk_term_pc fid b) (blk_term_id b) (blk_terminator b))
+    ,
+      CFG_fun_has_block CFG fid b.
+
 
 Definition CFG_fun_has_blocks (CFG:mcfg) (fid:function_id) (bs:list block) : Prop :=
   Forall (fun b => CFG_fun_has_block CFG fid b /\ CFG_fun_has_terminator_lbls CFG fid (snd (blk_term b))) bs.
